---
title: "Notes on generation interval"
output: pdf_document
---

Define survival function as follows:

$$
s_i(a) = \begin{cases}
\exp(- \beta a), \qquad a < r_i\\
\exp(- \beta r_i)
\end{cases}
$$

Define the probability that an infected person is still in the state, $\varphi$:

$$
\varphi_i(a) = \begin{cases}
1, \qquad a < r_i \\
0
\end{cases}
$$

Define

$$
l_i(a) = \varphi_i (a) s_i (a) = \begin{cases}
\exp(- \beta a), \qquad a < r_i\\
0
\end{cases}
$$

Now assume that we have exponentially distributed infectious period with mean $\gamma$ to get

$$
\begin{aligned}
\bigg< \exp(-\beta a)\bigg>_i &= \int_a^\infty \exp(-\beta a) \gamma \exp(-\gamma t) dt \\
&= \exp(-(\beta + \gamma) a)
\end{aligned}
$$

Normalizing this, we get 

$$
g(a) = (\beta + \gamma) \exp(- (\beta + \gamma) a)
$$

Let's do SEIR. Survival function:

$$
\begin{aligned}
s_i(a) = \begin{cases}
1, \qquad &a < m_i\\
\exp(-\beta(a - m_i)), \qquad &m_i \leq a < m_i + r_i\\
\exp(-\beta r_i)
\end{cases}
\end{aligned}
$$

Similarly, define

$$
\begin{aligned}
l_i(a) = \begin{cases}
0, \qquad &a < m_i\\
\exp(-\beta(a - m_i)), \qquad &m_i \leq a < m_i + r_i\\
0
\end{cases}
\end{aligned}
$$

We have to consider following conditions:

$$
\begin{cases}
m_i < a\\
r_i > a - m_i
\end{cases}
$$

If latent and infectious periods have probability density function of $f_E$ and $f_I$, this is what we're interested in:

$$
\int_0^a f_E(s) \left(e^{-\beta(a - s)} \int_{a-s}^\infty f_I (t) dt \right) ds
$$

Now, assume that latent and infectious periods are exponentially distributed with mean $\sigma$ and $\gamma$.

$$
\begin{aligned}
&\int_0^a f_E(s) \left(e^{-\beta(a - s)} \int_{a-s}^\infty f_I (t) dt \right) ds\\
&= \int_0^a f_E(s) \left(e^{-\beta(a - s)} \int_{a-s}^\infty \gamma e^{-\gamma t} dt \right) ds\\
&= \int_0^a f_E(s) \left(e^{-\beta(a - s)} e^{-\gamma(a - s)} \right) ds\\
&= \int_0^a f_E(s) \left(e^{-(\beta + \gamma)(a - s)} \right) ds\\
&= e^{-(\beta + \gamma) a } \int_0^a \sigma e^{-\sigma s} e^{(\beta + \gamma) s } ds\\
&= \sigma e^{-(\beta + \gamma) a} \int_0^a  e^{(\beta + \gamma - \sigma) s } ds\\
&= \sigma (e^{- \sigma a} - e^{-(\beta + \gamma) a})/(\beta + \gamma - \sigma)\\
\end{aligned}
$$

And we need to normalize to get the following generation distribution:

$$
g(a) = \frac{\sigma (\beta + \gamma)}{\beta + \gamma - \sigma} (e^{- \sigma a} - e^{-(\beta + \gamma) a})
$$
